Fix syntax and sem up to it_sems_core
Add Hoare rule for assert

remove warning

patch relational_logic, admit hoare_logic

patch psem

restore proofs

proof of wint_word + remove_assert

link remove_assert in compiler

Add more proof for Hoare Logic

Add ocaml part for bigop and assertions

Add proof for hoare

WIP

Temp fix of a test

Fix tests

Fix tests

extension for exprs, assertions

extension for exprs, assertions (Ocaml)

backward proof of wint_int (include safety), needs cleanup

WIP

safe semantics with catch

finish wint_int_proof

Take withcatch into account in relational_logic

fix slh_lowering_proof

safety_proof.v

shared defs wint_int

lemmas in safety_shared

safety.v

sc_op2 fix

New EC model for safety and safety pass added to compiler

safety proofs update

moved lemma wint_int_proof

safety_proof prog

EC library proofs for safety lemmas

compiler/entry/commonCLI.ml
@@ -57,7 +57,7 @@ let parse_and_compile (type reg regx xreg rflag cond asm_op extra_op)
        and type rflag = rflag
        and type cond = cond
        and type asm_op = asm_op
-       and type extra_op = extra_op) ~wi2i pass file idirs =
+       and type extra_op = extra_op) ~wi2i ~safety pass file idirs =
   let _env, pprog, _ast =
     try Compile.parse_file Arch.arch_info ~idirs file with
     | Annot.AnnotationError (loc, code) ->
@@ -74,8 +74,15 @@ let parse_and_compile (type reg regx xreg rflag cond asm_op extra_op)
       hierror ~loc:(Lmore loc) ~kind:"typing error" "%s" code
   in
 
+  Format.eprintf "@[<v>Program before safety passes:@;%a@.@]" 
+  (Printer.pp_prog ~debug:true Arch.reg_size Arch.asmOp) prog;
+
   let prog =
     if not wi2i then prog else Compile.do_wint_int (module Arch) prog
+  in 
+
+  let prog =
+    if not safety then prog else Compile.create_safety_asserts (module Arch) prog
   in
 
   let prog =
